---
tags:
  - notes
  - methods
  - topic
---
## Remember

### The Log function
$3^x = 81$
$Log_3 81 = x \rightarrow Log_3 364 = x = 4$ 

### Log Laws
- $a^m = n \rightarrow log_a n = m$ 
- $log_a (m) + log_a (n) = log_a (mn)$ 
- $log_a (m) - log_a (n) = log_a(\frac{m}{n})$
- $log_(a) a = 1$ 
- $log_a (1) = 0$ 
- $Log_a (0) \rightarrow undefined$ 
- $log_a (-m) \rightarrow \space non \space real \space number$ 
- $log_a (m^n) = nlog_a (m)$ 

## The Natural Logarithm
The natural logarithm, "ln" is defined as $\ln = log_e$  


## Examples
1. 
$log _2 (32) = log_2 (2^5) = 5 \times log_2 (2) = 5$


3. 
$log_{10} (5) + 2 \times log_{10} (7)$
$=log_{10} (5) + log_{10} (7^2) = log_{10} (245)$


4. 
$log_2 (2x+1) = 4$
$= 2^4 = 2x+1 = 16 \rightarrow x = \frac{17}{2} = 8.5$ 


5. $log_e(e^2) = 2 \times log_e e = 2$ 

6. 
$ln (x) = 3$
$e^3 = x$ 

7. 
$\ln (x-1) + \ln (x+2) = \ln (6x-8)$ 

$\ln [(x-1)(x+2)] = \ln (6x+8)$

$(x-1)(x+2) = 6x-8$

$x^2 - 5x + 6 = 0$ 

$(x-2)(x-3) = 0 \therefore x=2, \space or \space x=3$ 

8. 
$\ln (2z-1) - \ln (x-1) = 4$
$\ln \frac{2x-1}{x-1} = 4$
$e^4 = \frac {2x-1}{x-1}$ 
$e^4 \times (x-1) = 2x-1$ 
$1-e^4 = 2x-e^4 \times x$
$1-e^4 = (2-e^4) x$
$x = \frac{1-e^4}{2-e^4}$






























