---
tags:
  - methods
  - notes
  - topic
---
## Examples
1. 
$$y=x^{\frac{1}{1}} \: \: \rightarrow \: \: \frac{dy}{dx} = \frac{1}{3} \times x^{\frac{-2}{3}} = \frac{1}{3x^{\frac{2}{3}}}$$
2. 
$$y=5 \sqrt{x} =5x^\frac{1}{2} \: \: \rightarrow \: \:\frac{dy}{dx} = \frac{5}{2} x ^{\frac{1}{2}} = \frac{5}{2\sqrt{x}}$$
3. 
$$f(x) = \frac{6}{7\sqrt[3]{x^5}} = \frac{6}{7}x^{\frac{-5}{3}} \: \: \rightarrow \: \: -\frac{30}{21} x ^{\frac{-8}{3}} = \frac{-10}{7x^{\frac{8}{3}}} = \frac{-10}{7\sqrt[5]{x^8}}$$
4. 
$$h(x) \sqrt{x^2 - 5}... \: \:  \textrm{using chain rule}$$
$$h'(x)=\frac{1}{2}(x^2-5)^{\frac{-1}{2}} \times 2x = \frac{x}{\sqrt{x^2 - 5}}
$$







